\documentclass{article}
\usepackage{graphicx}
\usepackage{amsmath}
\usepackage{ dsfont }

\begin{document}
Tameez Latib


----

1. 

$$C = 
 \begin{bmatrix}
    1 & 2 & 3 & 4 \\
    2 & 5 & 7 & 9 \\
    3 & 7 & 11 & 14 \\
    4 & 9 & 14 & 19
\end{bmatrix}
$$

We want to find the LU factorization, so first we pivot on $C_{11}$:

$$C_1 = L_1C$$

Where 
$$L_1 = 
\begin{bmatrix}
    1 & 0 & 0 & 0 \\
    -2 & 1 & 0 & 0 \\
    -3 & 0 & 1 & 0 \\
    -4 & 0 & 0 & 1
\end{bmatrix}
$$

So that 
$$C_1 =  
\begin{bmatrix}
    1 & 2 & 3 & 4 \\
    0 & 1 & 1 & 1 \\
    0 & 1 & 2 & 2 \\
    0 & 1 & 2 & 3
\end{bmatrix}
$$

And now we pivot on $(C_1)_{22}$: 

$$C_2 = L_2C_1$$

Where 
$$L_2 = 
\begin{bmatrix}
    1 & 0 & 0 & 0 \\
    0 & 1 & 0 & 0 \\
    0 & -1 & 1 & 0 \\
    0 & -1 & 0 & 1
\end{bmatrix}
$$

So that 
$$C_2 =  
\begin{bmatrix}
    1 & 2 & 3 & 4 \\
    0 & 1 & 1 & 1 \\
    0 & 0 & 1 & 1 \\
    0 & 0 & 1 & 2
\end{bmatrix}
$$


And now we pivot on $(C_2)_{33}$: 

$$C_3 = L_3C_2$$

Where 
$$L_3 = 
\begin{bmatrix}
    1 & 0 & 0 & 0 \\
    0 & 1 & 0 & 0 \\
    0 & 0 & 1 & 0 \\
    0 & 0 & -1 & 1
\end{bmatrix}
$$

So that 
$$C_3 =  
\begin{bmatrix}
    1 & 2 & 3 & 4 \\
    0 & 1 & 1 & 1 \\
    0 & 0 & 1 & 1 \\
    0 & 0 & 0 & 1
\end{bmatrix}
$$

Now we have that $U = C_3$ and $L = (L_3L_2L_1)^{-1} = L_1^{-1}L_2^{-1}L_3^{-1}$

$$L = 
\begin{bmatrix}
    1 & 0 & 0 & 0 \\
    2& 1 & 0 & 0 \\
    3 & 1 & 1 & 0 \\
    4 & 1 & 1 & 1
\end{bmatrix}
$$

$$U
\begin{bmatrix}
    1 & 2 & 3 & 4 \\
    0 & 1 & 1 & 1 \\
    0 & 0 & 1 & 1 \\
    0 & 0 & 0 & 1
\end{bmatrix}
$$


2. $A \in \mathds{R}^{n \times n}$ is strictly diagonally dominant, then if $A = D - R$, where D is a diagonal matrix, then

a. Show $||D^{-1}R||_{\infty} < 1$

Since A is strictly diagonally dominant, $$ |D_{ii}|  = |A_{ii}|  > \sum^n_{j=1, j \ne i}|A_{ij}| = \sum^n_{j=1, j \ne i} |R_{ij}| $$

for all $i$

Therefore, $$\sum^n_{j=1, j \ne i} |(D^{-1}R)_{ij}| = \sum^n_{j=1, j \ne i}|(D^{-1})_{ii}R_{ij}| = \frac{\sum^n_{j=1, j \ne i}|R_{ij}|}{D_{ii}} < 1   $$ 

for all $i$

Also note that $(D^{-1}R)_{ii} = 0$, so we then have

$$\sum^n_{j=1} |(D^{-1}R)_{ij} | < 1$$ 

for all $i$, so $||D^{-1}R||_{\infty} < 1$


b. Show the iteration 
$$x_{k+1} = D^{-1}Rx_k + D^{-1}b$$

converges and converges to the solution of $Ax = b$

Since $||D^{-1}R||_{\infty} < 1$, we can apply fixed point theorem element-wise on $x_k$, 

$(x_k)_i = 

\end{document}
